secure_api/merkle_tree/MerkleTree.New.Low.Hashes.fst
@@ -10,3 +10,4 @@ open Lib.IntTypes
 type hash_size_t = n:uint32_t{n > 0ul}
 type hash (#hsz:hash_size_t) = b:B.buffer uint8 { B.len b = hsz \/ B.g_is_null b }
 
+
